Better with primitives actually implementedt

src/rocq/Semantics/Memory.v
@@ -82,6 +82,9 @@ Definition fresh_addr {S A P}     : memS S A P A := fun σ => Mfresh_addr σ (fu
 Definition fresh_prov {S A P}     : memS S A P P := fun σ => Mfresh_prov σ (fun p => ret (σ,p)). 
 
 (*** Internal state of memory *)
+(* TODO: MemoryModelPrimitives feels fairly reasonable, but what is exposed
+   in MemoryModelState feels quite random.
+ *)
 Class MemoryModelState {Pa : Params} :=
   {
     
@@ -109,8 +112,15 @@ Class MemoryModelState {Pa : Params} :=
 
   }.
 
-Definition memM {Pa : Params} {MMS : @MemoryModelState Pa} :=
-  memS state addr provenance.
+Section MemM.
+  Context {Pa : Params} {MMS : @MemoryModelState Pa}.
+
+  Definition memM := memS state addr provenance.
+
+  Definition get_state  : memM state := fun s => ret (s,s).
+  Definition get_memory : memM memory_stack := fun s => ret (s, state_get_memory s).
+
+End MemM.
 
 (*** Primitives on memory *)
 Class MemoryModelPrimitives {Pa : Params} :=
@@ -239,7 +249,7 @@ Section MemoryModel.
       let byte := MByte (DVALUE_I 8 val) (DTYPE_I 8) 0 in
       write_bytes dst (repeatN (Z.to_N len) byte).
 
-  Definition handle_memory : MemoryE ~> memM :=
+  Definition handle_memoryM : MemoryE ~> memM :=
     fun T m =>
       match m with
       | MemPush => mempush
@@ -308,8 +318,7 @@ Section Implementation.
         state_provenance : provenance;
       }.
 
-  (* #[refine] Instance MemoryModelPrimitivesV {Pa : Params} : MemoryModelState := *)
-  Instance MemoryModelPrimitivesV : @MemoryModelState Pa :=
+  Instance MemoryModelStateV : @MemoryModelState Pa :=
     {|
       memory_stack := Memory_stack ;
       state := State ;
@@ -326,6 +335,206 @@ Section Implementation.
       initial_heap := heap_empty ;
     |}.
 
+  (** Operations on memory *)
+  Definition read_byte_raw_mem (mem : memory) (phys_addr : Z) : option byte :=
+    IM.find phys_addr mem.
+  Definition set_byte_raw_mem  (mem : memory) (phys_addr : Z) (byte : byte) : memory :=
+    IM.add phys_addr byte mem.
+  Definition next_key_mem (mem : memory) : Z :=
+    next_key mem.
+
+  (** Add block to memory with a given allocation id *)
+  Definition memory_bytes_to_bytes
+    (aid : allocationId) (bytes : list memory_byte) : list byte :=
+    map (fun b => (b, aid)) bytes.
+
+  (* Register a concrete address in a frame *)
+  Definition add_to_frame (m : memory_stack) (k : addr) : memory_stack :=
+    let '(mkMemoryStack m s h) := m in
+    match s with
+    | Singleton f => mkMemoryStack m (Singleton (k :: f)) h
+    | Snoc s f => mkMemoryStack m (Snoc s (k :: f)) h
+    end.
+
+  (* Register a list of concrete addresses in a frame *)
+  Definition add_all_to_frame (ks : list addr) (m : memory_stack) : memory_stack
+    := fold_left (fun ms k => add_to_frame ms k) ks m.
+
+  (* Register a ptr with the heap *)
+  Definition add_to_heap (m : memory_stack) (root : addr) (ptr : addr) : memory_stack :=
+    let '(mkMemoryStack m s h) := m in
+    let h' := add_with (ptr_to_int root) ptr ret cons h in
+    mkMemoryStack m s h'.
+
+  (* Register a list of concrete addresses in the heap *)
+  Definition add_all_to_heap' (m : memory_stack) (root : addr) (ks : list addr) : memory_stack
+    := fold_left (fun ms k => add_to_heap ms root k) ks m.
+
+  Definition add_all_to_heap (ks : list addr) (m : memory_stack) : memory_stack
+    := match ks with
+       | [] => m
+       | (root :: _) =>
+           add_all_to_heap' m root ks
+       end.
+
+  Definition get_frame_stack : memM Framestack :=
+    fun s => ret (s,Memory_stack_frame_stack (state_get_memory s)).
+  Definition get_frame : memM Frame :=
+    fs <- get_frame_stack ;;
+    match fs with
+    | Singleton f | Snoc _ f => ret f
+    end. 
+  Definition get_mem : memM memory :=
+    fun s => ret (s,Memory_stack_memory (state_get_memory s)).
+  Definition get_framestack : memM Framestack :=
+    fun s => ret (s,Memory_stack_frame_stack (state_get_memory s)).
+  
+  Definition app_state : (state -> state) -> memM unit :=
+    fun f s => ret (f s, tt).
+  Definition app_mem_stack : (Memory_stack -> Memory_stack) -> memM unit :=
+    fun f s =>
+      ret ({| state_memory_stack := f s.(state_memory_stack) ;
+             state_provenance := state_provenance s |},tt).
+  Definition upd_mem_stack (m : Memory_stack) : memM unit := app_mem_stack (fun _ => m).
+  Definition app_mem : (memory -> memory) -> memM unit :=
+    fun f s =>
+      ret ({| state_memory_stack :=
+               {| Memory_stack_memory     := f s.(state_memory_stack).(Memory_stack_memory) ;
+                 Memory_stack_frame_stack := s.(state_memory_stack).(Memory_stack_frame_stack);
+                 Memory_stack_heap        := s.(state_memory_stack).(Memory_stack_heap)
+               |};
+             state_provenance := state_provenance s |},tt).
+  Definition upd_mem (m : memory) : memM unit := app_mem (fun _ => m).
+  Definition app_frame_stack : (Framestack -> Framestack) -> memM unit :=
+    fun f s =>
+      ret ({| state_memory_stack :=
+               {| Memory_stack_memory     := s.(state_memory_stack).(Memory_stack_memory) ;
+                 Memory_stack_frame_stack := f s.(state_memory_stack).(Memory_stack_frame_stack);
+                 Memory_stack_heap        := s.(state_memory_stack).(Memory_stack_heap)
+               |};
+             state_provenance := state_provenance s |},tt).
+  Definition upd_frame_stack (fs : Framestack) : memM unit := app_frame_stack (fun _ => fs).
+  Definition app_frame_stack_eob : (Framestack -> EOB Framestack) -> memM unit :=
+    fun f =>
+      fs <- get_framestack ;;
+      f' <- lift (f fs) ;;
+      upd_frame_stack f'.
+  
+  Definition next_key : memM Z :=
+    m <- get_mem ;;
+    ret (next_key_mem m).
+
+  Definition push_frame_stack (f : Frame) (fs : Framestack) : Framestack :=
+    Snoc fs f.
+  Definition pop_frame_stack (fs : Framestack) : EOB Framestack :=
+    match fs with
+    | Singleton f => raise_error "Last frame, cannot pop."%string
+    | Snoc s f => ret s
+    end.
+
+  Definition read_byte_raw (msg : string) (phys_addr : Z) : memM byte :=
+    fun s =>
+      match read_byte_raw_mem (Memory_stack_memory (state_get_memory s)) phys_addr with
+      | Some b => ret (s,b)
+      | None => Mub msg
+      end.
+  
+  Definition set_byte_raw (phys_addr : Z) (byte : byte) : memM unit :=
+    m <- get_mem ;;
+    upd_mem (set_byte_raw_mem m phys_addr byte).
+
+  (** Add block to memory with a given allocation id *)
+  Definition add_block (aid : allocationId) (ptr : addr)
+    (ptrs : list addr) (init_bytes : list memory_byte) : memM unit :=
+    let mem_bytes := memory_bytes_to_bytes aid init_bytes in
+    m <- get_mem;;
+    upd_mem (add_all_index mem_bytes (ptr_to_int ptr) m).
+
+  (** Add pointers to the stack frame *)
+  Definition add_ptrs_to_frame (ptrs : list addr) : memM unit :=
+    app_mem_stack (add_all_to_frame ptrs).
+  
+  Definition add_ptrs_to_heap (ptrs : list addr) : memM unit :=
+    app_mem_stack (add_all_to_heap ptrs).
+ 
+  (** Add a block of bytes to memory, and register it in the current stack frame. *)
+  Definition add_block_to_stack (aid : allocationId) (ptr : addr)
+    (ptrs : list addr) (init_bytes : list memory_byte) : memM unit :=
+    add_block aid ptr ptrs init_bytes;;
+    add_ptrs_to_frame ptrs.
+
+  (** Add a block of bytes to memory, and register it in the heap. *)
+  (* Should we make sure ptr (the root) is added even if ptrs is empty? *)
+  Definition add_block_to_heap (aid : allocationId) (ptr : addr)
+    (ptrs : list addr) (init_bytes : list memory_byte) : memM unit :=
+    add_block aid ptr ptrs init_bytes;;
+    add_ptrs_to_heap ptrs.
+
+  Definition Read_byte (ptr : addr) : memM memory_byte :=
+    let addr := ptr_to_int ptr in
+    let pr := address_provenance ptr in
+    '(byte,aid) <- read_byte_raw "Reading from unallocated memory." addr;;
+    if access_allowed pr aid
+    then ret byte
+    else mub ("Read from memory with invalid provenance").
+
+  (** Writes *)
+  Definition Write_byte (ptr : addr) (byte : memory_byte) : memM unit :=
+    let addr := ptr_to_int ptr in
+    let pr := address_provenance ptr in
+    '(_,aid) <- read_byte_raw "Writing to unallocated memory" addr ;;
+    if access_allowed pr aid
+    then set_byte_raw addr (byte,aid)
+    else mub "Trying to write to memory with invalid provenance".
+
+  Definition get_free_block (len : nat) (pr : provenance) : memM (addr * list addr) :=
+    let aid := provenance_to_allocation_id pr in
+    addr <- next_key ;;
+    ptr <- lift (int_to_ptr addr (allocation_id_to_prov aid)) ;;
+    ptrs <- lift (get_consecutive_ptrs ptr len);;
+    ret (ptr,ptrs).
+
+  Definition Allocate_bytes_with_pr (init_bytes : list memory_byte) (pr : provenance) : memM addr :=
+    let len := List.length init_bytes in
+    let aid := provenance_to_allocation_id pr in
+    '(ptr, ptrs) <- get_free_block len pr;;
+    add_block_to_stack aid ptr ptrs init_bytes;;
+    ret ptr.
+
+  (** Heap allocation *)
+  Definition Malloc_bytes_with_pr (init_bytes : list memory_byte) (pr : provenance) : memM addr :=
+    let len := List.length init_bytes in
+    let aid := provenance_to_allocation_id pr in
+    '(ptr, ptrs) <- get_free_block len pr;;
+    add_block_to_heap aid ptr ptrs init_bytes;;
+    ret ptr.
+
+  Definition Mempush : memM unit :=
+    app_frame_stack (push_frame_stack initial_frame).
+
+  Definition free_byte (b : Z) (m : memory) : memory :=
+    delete b m.
+
+  Definition free_frame_memory (f : Frame) (m : memory) : memory :=
+    fold_left (fun m key => free_byte (ptr_to_int key) m) f m.
+
+  (** Stack free *)
+  Definition Mempop : memM unit :=
+    f <- get_frame ;;
+    app_frame_stack_eob pop_frame_stack;;
+    app_mem (free_frame_memory f).
+
+  Instance MemoryModelPrimitivesV : @MemoryModelPrimitives Pa :=
+    {|
+      mm_state := MemoryModelStateV ;
+      read_byte := Read_byte ;
+      write_byte := Write_byte ;
+      allocate_bytes_with_pr := Allocate_bytes_with_pr ;
+      malloc_bytes_with_pr := Malloc_bytes_with_pr ;
+      mempush := Mempush ;
+      mempop := Mempop ;
+    |}.
+  
 End Implementation.
 
 
