src/rocq/Handlers/Memory.v
@@ -25,3 +25,37 @@ From Vellvm Require Import
 From QuickChick Require Import Show.
 
 
+Section withParams.
+  Context {Pa : Params}.
+
+  Existing Instance MemoryModelPrimitivesV.
+  
+  Definition handle_memory {E} (h : memM ~> itree E) : MemoryE ~> itree E.
+    Set Printing Implicit.
+    refine (fun T e => h _ _).
+    refine (@handle_memoryM Pa (@MemoryModelPrimitivesV Pa) T _).
+    refine (fun T e => h _ (handle_memoryM e)).
+    fun T m =>
+      match m with
+      | MemPush => mempush
+      | MemPop => mempop
+      | Alloca t n align =>
+          addr <- allocate_dtyp t n;;
+          ret (DVALUE_Addr addr)
+      | Load t a =>
+          match a with
+          | DVALUE_Addr a =>
+              read_dvalue t a
+          | _ => mub "Loading from something that isn't an address."
+          end
+      | Store t a v =>
+          match a with
+          | DVALUE_Addr a =>
+              write_dvalue t a v
+          | _ => mub "Writing something to somewhere that isn't an address."
+          end
+      end.
+
+ 
+End withParams.
+
